generated high-level proofs
git-svn-id: https://webdav.seas.upenn.edu/svn/sol/vol@3450 eef5ea85-cc2e-0410-bd84-0fae1f012da8

src/Transforms/promotable_props.v
@@ -16,6 +16,8 @@ Require Import Maps.
 Require Import mem2reg.
 Require Import opsem_props.
 
+Definition DGVMap := @Opsem.GVsMap DGVs.
+
 Record PhiInfo := mkPhiInfo {
   PI_f: fdef;
   PI_rd: list l;
@@ -41,6 +43,1406 @@ reachablity_analysis f = Some rd /\
 succs = successors f /\
 preds = make_predecessors succs /\
 newids = fst (gen_fresh_ids rd (getFdefLocs f)).
+
+(* wf_global and wf_globals are copied from sb_ds_gv_inject.v 
+   We should move the invariant to memory model. *)
+Fixpoint wf_global (maxb:Values.block) (gv:GenericValue) 
+  : Prop :=
+match gv with
+| nil => True
+| (Vptr b _,_)::gv' => b <= maxb /\ wf_global maxb gv'
+| _::gv' => wf_global maxb gv'
+end.
+
+Fixpoint wf_globals maxb (gl:GVMap) : Prop :=
+match gl with
+| nil => True
+| (_,gv)::gl' => wf_global maxb gv /\ wf_globals maxb gl'
+end.
+
+Fixpoint no_alias_with_blk (gvs:GenericValue) (blk:Values.block) : Prop :=
+match gvs with
+| nil => True
+| (Vptr b _,_)::gvs' => b <> blk /\ no_alias_with_blk gvs' blk
+| _::gvs' => no_alias_with_blk gvs' blk
+end.
+
+Fixpoint no_alias (gvs1 gvs2:GenericValue) : Prop :=
+match gvs2 with
+| nil => True
+| (Vptr b _,_)::gvs2' => no_alias_with_blk gvs1 b /\ no_alias gvs1 gvs2'
+| _::gvs2' => no_alias gvs1 gvs2'
+end.
+
+Definition wf_non_alloca_GVs (pinfo:PhiInfo) (id1:id) (gvs1 gvsa:GenericValue) 
+  : Prop :=
+(if (id_dec id1 (PI_id pinfo)) then True else no_alias gvs1 gvsa).
+
+Definition wf_alloca_GVs (maxb:Values.block) (pinfo:PhiInfo) TD Mem 
+  (gvsa:GenericValue) (als:list Values.block) : Prop :=
+(exists mb, gvsa = ($ (blk2GV TD mb) # (typ_pointer (PI_typ pinfo)) $) /\
+   In mb als /\ maxb < mb) /\
+(forall gptr gvs1, 
+   mload TD Mem gptr (PI_typ pinfo) (PI_align pinfo) = Some gvs1 ->
+   no_alias gvs1 gvsa) /\
+exists gv,
+  mload TD Mem gvsa (PI_typ pinfo) (PI_align pinfo) = Some gv.
+
+Definition wf_defs (maxb:Values.block) (pinfo:PhiInfo) TD M (lc:DGVMap) 
+  (ids0:list atom) (als:list Values.block) : Prop :=
+forall gvsa
+  (Hinp: In (PI_id pinfo) ids0)
+  (Hlkp: lookupAL _ lc (PI_id pinfo) = Some gvsa),
+  wf_alloca_GVs maxb pinfo TD M gvsa als /\
+  (forall id0 gvs0 
+   (Hin0: In id0 ids0) 
+   (Hlk0: lookupAL _ lc id0 = Some gvs0),
+   wf_non_alloca_GVs pinfo id0 gvs0 gvsa).
+
+Definition mk_gptr (blk:Values.block) (ofs:int32) : GenericValue :=
+((Vptr blk ofs, AST.Mint 31)::nil).
+
+Definition wf_lc M lc : Prop :=
+(forall id0 blk ofs, 
+  lookupAL _ lc id0 = Some (mk_gptr blk ofs) -> blk < Mem.nextblock M).
+
+(* Except domination property, the other properties are the same for a lot of 
+   proofs, we should prove them all for once. Or, we do not need to use them
+   in this invariant, we can assume the invariant in opsem_wf, which is 
+   preserved *)
+Definition wf_ExecutionContext (maxb:Values.block) (pinfo:PhiInfo) TD M 
+  (ec:Opsem.ExecutionContext) : Prop :=
+let '(Opsem.mkEC f b cs tmn lc als) := ec in
+(if (fdef_dec (PI_f pinfo) f) then 
+  match cs with
+  | nil => 
+    match inscope_of_tmn f b tmn with
+    | Some ids => wf_defs maxb pinfo TD M lc ids als
+    | None => False
+    end
+  | c::_ =>
+    match inscope_of_cmd f b c with
+    | Some ids => wf_defs maxb pinfo TD M lc ids als
+    | None => False
+    end
+  end 
+else True)
+/\ wf_lc M lc.
+
+Definition wf_ECStack_head_tail (maxb:Values.block) (pinfo:PhiInfo) TD M 
+  (lc:DGVMap) (ecs':list (fdef * DGVMap)) : Prop :=
+  forall ec0 gvsa, 
+    In ec0 ecs' ->
+    fst ec0 = PI_f pinfo ->
+    lookupAL _ (snd ec0) (PI_id pinfo) = Some gvsa ->
+    (forall id1 gvs1, 
+      lookupAL _ lc id1 = Some gvs1 -> 
+      no_alias gvs1 gvsa) /\
+    (forall gptr gvs1, 
+      mload TD M gptr (PI_typ pinfo) (PI_align pinfo) = Some gvs1 -> 
+      no_alias gvs1 gvsa).
+
+Fixpoint wf_ECStack (maxb:Values.block) (pinfo:PhiInfo) TD M (ecs:Opsem.ECStack)
+  : Prop :=
+match ecs with
+| nil => True
+| ec::ecs' => 
+    wf_ExecutionContext maxb pinfo TD M ec /\
+    wf_ECStack maxb pinfo TD M ecs' /\
+    wf_ECStack_head_tail maxb pinfo TD M (Opsem.Locals ec) 
+      (List.map (fun ec => let '(Opsem.mkEC f _ _ _ lc _) := ec in (f, lc)) ecs')
+end.
+
+Definition wf_Mem maxb (td:targetdata) (M:mem) : Prop :=
+(forall gptr ty al blk ofs, 
+  mload td M gptr ty al = Some (mk_gptr blk ofs) -> blk < Mem.nextblock M) /\
+maxb < Mem.nextblock M.
+
+Definition wf_als maxb M (als: list Values.block) : Prop :=
+NoDup als /\ (forall al, In al als -> maxb < al < Mem.nextblock M).
+
+Definition wf_State (maxb:Values.block) (pinfo:PhiInfo) (cfg:OpsemAux.Config) 
+  (S:Opsem.State) : Prop :=
+let '(OpsemAux.mkCfg _ td _ _ _ ) := cfg in
+let '(Opsem.mkState ecs M) := S in
+wf_ECStack maxb pinfo td M ecs /\
+wf_als maxb M 
+  (flat_map (fun ec => let '(Opsem.mkEC _ _ _ _ _ als) := ec in als) ecs) /\
+wf_Mem maxb td M.
+
+Lemma wf_defs_eq : forall maxb pinfo TD M lc ids1 ids2 als,
+  AtomSet.set_eq _ ids1 ids2 ->
+  wf_defs maxb pinfo TD M lc ids1 als ->
+  wf_defs maxb pinfo TD M lc ids2 als.
+Proof.
+  intros. unfold wf_defs in *. intros.
+  destruct H as [H1 H2]. eauto.
+  apply H0 in Hlkp; auto.
+    destruct Hlkp as [J1 J2].
+    split; auto.
+Qed.
+
+Definition wf_GVs (maxb:Values.block)(pinfo:PhiInfo)(TD:targetdata)(M:mem)
+  (lc:DGVMap)(ids1:list id)(als:list Values.block)(id1:id)(gv1:GVsT DGVs)
+  : Prop :=
+  (forall gvsa,
+     In (PI_id pinfo) ids1 ->
+     lookupAL _ lc (PI_id pinfo) = Some gvsa ->
+     no_alias gv1 gvsa) /\
+  (id1 = (PI_id pinfo) ->
+     (forall id0 gvs0,
+        lookupAL (GVsT DGVs) lc id0 = ret gvs0 ->
+        no_alias gvs0 gv1) /\
+     wf_alloca_GVs maxb pinfo TD M gv1 als).
+
+Lemma wf_defs_updateAddAL: forall maxb pinfo TD M lc' ids1 ids2 i1 gv1 als
+  (HwfDef: wf_defs maxb pinfo TD M lc' ids1 als)
+  (Heq: AtomSet.set_eq _ (i1::ids1) ids2)
+  (Hwfgvs: wf_GVs maxb pinfo TD M lc' ids1 als i1 gv1),
+  wf_defs maxb pinfo TD M (updateAddAL _ lc' i1 gv1) ids2 als.
+Proof.
+  intros. unfold wf_defs. intros.
+  destruct Hwfgvs as [Hwfgvs1 Hwfgvs2].
+  destruct Heq as [Hinc1 Hinc2].
+  apply Hinc2 in Hinp. simpl in Hinp.
+  destruct (eq_dec i1 (PI_id pinfo)); subst.
+    rewrite lookupAL_updateAddAL_eq in Hlkp.
+    inv Hlkp.
+    destruct Hwfgvs2 as [J1 J2]; auto.
+    split; auto.
+      intros. unfold wf_non_alloca_GVs.
+      apply Hinc2 in Hin0. simpl in Hin0.
+      destruct (id_dec id0 (PI_id pinfo)); subst; auto.
+      rewrite <- lookupAL_updateAddAL_neq in Hlk0; auto.
+      apply J1 in Hlk0; auto.
+
+    clear Hwfgvs2.
+    rewrite <- lookupAL_updateAddAL_neq in Hlkp; auto.
+    destruct Hinp as [EQ | Hinp]; subst; try congruence.
+    assert (Hlkp':=Hlkp).
+    apply HwfDef in Hlkp; auto.
+    destruct Hlkp as [J1 J2].
+    split; auto.
+      intros.
+      destruct (id_dec i1 id0); subst.
+        rewrite lookupAL_updateAddAL_eq in Hlk0.
+        inv Hlk0. apply Hwfgvs1 in Hlkp'; auto.
+        unfold wf_non_alloca_GVs.
+        destruct (id_dec id0 (PI_id pinfo)); subst; auto.
+
+        rewrite <- lookupAL_updateAddAL_neq in Hlk0; auto.
+        apply Hinc2 in Hin0.
+        simpl in Hin0.
+        destruct Hin0 as [Hin0 | Hin0]; subst; try congruence; auto.
+Qed.
+
+Lemma free_preserves_mload_inv: forall TD Mem' gptr ty al gvsa Mem mptr0
+  (H1 : mload TD Mem' gptr ty al = ret gvsa)
+  (H2 : free TD Mem mptr0 = ret Mem'),
+  mload TD Mem gptr ty al = ret gvsa.
+Proof.
+  intros.
+  apply mload_inv in H1.
+  destruct H1 as [b [ofs [m [mc [J1 [J2 J3]]]]]]; subst.
+  unfold mload. simpl. rewrite J2.
+  apply free_inv in H2.
+  destruct H2 as [blk' [ofs' [hi [lo [J4 [J5 [J6 J7]]]]]]].
+  admit. (* Mem Props *)
+Qed.
+
+Lemma free_preserves_wf_ECStack_head_tail : forall maxb pinfo TD M M' lc mptr0
+  (Hfree: free TD M mptr0 = ret M') ECs 
+  (Hwf: wf_ECStack_head_tail maxb pinfo TD M lc ECs),
+  wf_ECStack_head_tail maxb pinfo TD M' lc ECs.
+Proof.
+  unfold wf_ECStack_head_tail.
+  intros.
+  eapply Hwf in H1; eauto.
+  destruct H1 as [J1 J2].
+  split; auto.
+    intros.
+    eapply free_preserves_mload_inv in H1; eauto.
+Qed.
+
+Lemma free_preserves_wf_lc: forall TD Mem' Mem mptr0 lc
+  (H2 : free TD Mem mptr0 = ret Mem')
+  (Hwf: wf_lc Mem lc),
+  wf_lc Mem' lc.
+Proof.
+  unfold wf_lc.
+  intros.
+  apply Hwf in H.
+  apply free_inv in H2.
+  destruct H2 as [blk' [ofs' [hi [lo [J4 [J5 [J6 J7]]]]]]].
+  admit. (* Mem Props *)
+Qed.
+(*
+Lemma free_allocas_preserves_mload: forall TD Mem als Mem' t al gv mb
+  (H0 : ~ In mb als)
+  (H1 : free_allocas TD Mem als = ret Mem')
+  (H2 : mload TD Mem ($ blk2GV TD mb # typ_pointer t $) t al = ret gv),
+  mload TD Mem' ($ blk2GV TD mb # typ_pointer t $) t al = ret gv.
+Admitted.
+*)
+
+Definition wf_use (pinfo:PhiInfo) (ids0:list id) (v:value) :=
+used_in_value (PI_id pinfo) v = false /\
+match v with
+| value_const _ => True
+| value_id vid => In vid ids0
+end.
+
+Lemma wf_globals_disjoint_with_runtime_alloca: forall maxb gl g td c0 mb t
+  (Hwfg: wf_globals maxb gl)
+  (Hc2g : ret g = @Opsem.const2GV DGVs td gl c0)
+  (Hle: maxb < mb),
+  no_alias g ($ blk2GV td mb # typ_pointer t $).
+Admitted.
+
+Lemma free_preserves_mload: forall TD Mem Mem' t al gv gptr gvsa
+  (H0 : no_alias gptr gvsa)
+  (H1 : free TD Mem gptr = ret Mem')
+  (H2 : mload TD Mem gvsa t al = ret gv),
+  mload TD Mem' gvsa t al = ret gv.
+Proof.
+  intros.
+  apply free_inv in H1.
+  destruct H1 as [blk [ofs [hi [lo [J4 [J5 [J6 J7]]]]]]].
+Admitted.
+
+Lemma free_preserves_wf_defs : forall maxb pinfo TD M  
+  M' lc1 mptr0 mptrs gl v als ids0 lc2
+  (Hwfu: wf_use pinfo ids0 v)
+  (Hgetop: Opsem.getOperandValue TD v lc1 gl = ret mptrs)
+  (Hin: mptr0 @ mptrs)
+  (Hwflc: wf_lc M lc1) (Hwfgl: wf_globals maxb gl)
+  (Hfree: free TD M mptr0 = ret M')
+  (Hwf: wf_defs maxb pinfo TD M lc2 ids0 als),
+  wf_defs maxb pinfo TD M' lc2 ids0 als.
+Proof.
+  intros. unfold wf_defs. 
+  intros gvsa Hpindom Hlkp.
+  assert (Hlkp':=Hlkp).
+  apply Hwf in Hlkp'; auto.
+  destruct Hlkp' as [J1 J2].
+  split; auto.
+    destruct J1 as [J1 [J4 [gv J3]]].
+    split; auto.
+      split.
+        intros. eapply free_preserves_mload_inv in H; eauto.
+        clear J4. inv Hin.
+        assert (no_alias mptr0 gvsa) as J.
+          destruct Hwfu as [G1 G2].
+          destruct v; simpl in Hgetop.
+(*
+          apply J2 in Hgetop; auto.
+          unfold wf_non_alloca_GVs in Hgetop.
+          simpl in G1. 
+          destruct (id_dec i0 (PI_id pinfo)); subst; tinv G1; auto.
+
+          destruct J1 as [mb [J11 [J12 J13]]]; subst.
+          eapply wf_globals_disjoint_with_runtime_alloca; eauto.
+        exists gv. eapply free_preserves_mload; eauto.
+*)
+Admitted.
+
+Lemma free_preserves_wf_EC_tail : forall maxb pinfo TD M  
+  M' mptr0 mptrs gl v EC (Hwfpi: WF_PhiInfo pinfo) lc
+  (Hgetop: Opsem.getOperandValue TD v lc gl = ret mptrs)
+  (Hin: mptr0 @ mptrs)
+  (Hwflc: wf_lc M lc) (Hwfgl: wf_globals maxb gl)
+  (Hfree: free TD M mptr0 = ret M')
+  (Hwf: wf_ExecutionContext maxb pinfo TD M EC),
+  wf_ExecutionContext maxb pinfo TD M' EC.
+Proof.
+  destruct EC. simpl. intros.
+  destruct Hwf as [J1 J2].
+  eapply free_preserves_wf_lc in J2; eauto.
+  split; auto.
+    destruct (fdef_dec (PI_f pinfo) CurFunction); subst; auto.
+    destruct CurCmds.    
+      remember (inscope_of_tmn (PI_f pinfo) CurBB Terminator) as R.
+      destruct R; auto.
+      eapply free_preserves_wf_defs in Hfree; eauto.   
+        admit. (* v >> current pc && Hwfpi *)
+
+      remember (inscope_of_cmd (PI_f pinfo) CurBB c) as R.
+      destruct R; auto.
+      eapply free_preserves_wf_defs in Hfree; eauto.   
+        admit. (* v >> current pc && Hwfpi *)
+Qed.
+
+Lemma free_preserves_wf_ECStack : forall maxb pinfo TD M  
+  M' mptr0 mptrs gl v (Hwfpi: WF_PhiInfo pinfo) lc
+  (Hgetop: Opsem.getOperandValue TD v lc gl = ret mptrs)
+  (Hin: mptr0 @ mptrs)
+  (Hwflc: wf_lc M lc) (Hwfgl: wf_globals maxb gl)
+  (Hfree: free TD M mptr0 = ret M') ECs
+  (Hwf: wf_ECStack maxb pinfo TD M ECs),
+  wf_ECStack maxb pinfo TD M' ECs.
+Proof.
+  induction ECs; simpl; intros; auto.
+    destruct Hwf as [J1 [J2 J3]].
+    split.
+      eapply free_preserves_wf_EC_tail; eauto.
+    split; eauto.
+      eapply free_preserves_wf_ECStack_head_tail; eauto.
+Qed.
+
+Lemma free_preserves_wf_EC : forall maxb pinfo TD M  
+  M' lc mptr0 mptrs gl v F B id0 t als tmn cs
+  (Hgetop: Opsem.getOperandValue TD v lc gl = ret mptrs)
+  (Hin: mptr0 @ mptrs)
+  (Hwflc: wf_lc M lc) (Hwfgl: wf_globals maxb gl)
+  (Hfree: free TD M mptr0 = ret M') 
+  (HwfEC: wf_ExecutionContext maxb pinfo TD M 
+            {| Opsem.CurFunction := F;
+               Opsem.CurBB := B;
+               Opsem.CurCmds := insn_free id0 t v :: cs;
+               Opsem.Terminator := tmn;
+               Opsem.Locals := lc;
+               Opsem.Allocas := als |}),
+  wf_ExecutionContext maxb pinfo TD M'
+   {| Opsem.CurFunction := F;
+      Opsem.CurBB := B;
+      Opsem.CurCmds := cs;
+      Opsem.Terminator := tmn;
+      Opsem.Locals := lc;
+      Opsem.Allocas := als |}.
+Admitted.
+
+Lemma free_preserves_wf_Mem : forall maxb TD M M' lc mptr0 mptrs gl v
+  (Hgetop: Opsem.getOperandValue TD v lc gl = ret mptrs)
+  (Hin: mptr0 @ mptrs)
+  (Hwflc: wf_lc M lc) (Hwfgl: wf_globals maxb gl)
+  (Hfree: free TD M mptr0 = ret M') 
+  (Hwf: wf_Mem maxb TD M),
+  wf_Mem maxb TD M'.
+Admitted.
+
+Lemma free_preserves_wf_als : forall maxb TD M M' mptr0 als
+  (Hfree: free TD M mptr0 = ret M') 
+  (Hwf: wf_als maxb M als),
+  wf_als maxb M' als.
+Admitted.
+
+Lemma free_allocas_preserves_mload_inv: forall TD Mem' gptr ty al gvsa Mem als
+  (H1 : mload TD Mem' gptr ty al = ret gvsa)
+  (H2 : free_allocas TD Mem als = ret Mem'),
+  mload TD Mem gptr ty al = ret gvsa.
+Proof.
+Admitted.
+
+Lemma free_allocas_preserves_mload: forall TD Mem als Mem' t al gv mb
+  (H0 : ~ In mb als)
+  (H1 : free_allocas TD Mem als = ret Mem')
+  (H2 : mload TD Mem ($ blk2GV TD mb # typ_pointer t $) t al = ret gv),
+  mload TD Mem' ($ blk2GV TD mb # typ_pointer t $) t al = ret gv.
+Admitted.
+
+(* We need a generic proof for this one and the one for atom *)
+Lemma NoDup_disjoint : forall (l1 l2 : list Z) (i0 : Z),
+  NoDup (l1 ++ l2) -> In i0 l2 -> ~ In i0 l1.
+Admitted.
+
+Lemma free_allocas_preserves_wf_alloca: forall maxb pinfo TD Mem gvsa als0 als Mem',
+  wf_alloca_GVs maxb pinfo TD Mem gvsa als0 ->
+  NoDup (als ++ als0) ->
+  free_allocas TD Mem als = ret Mem' ->
+  wf_alloca_GVs maxb pinfo TD Mem' gvsa als0.
+Proof.
+  intros.
+  unfold wf_alloca_GVs in *.
+  destruct H as [J1 [J2 J3]].
+  split; auto.
+  split.
+    intros gptr gvs1 J.  
+    eapply free_allocas_preserves_mload_inv in J; eauto.
+
+    destruct J3 as [gv J3].
+    exists gv.
+    destruct J1 as [mb [J11 [J12 J13]]]; subst.
+    eapply free_allocas_preserves_mload; eauto.
+    eapply NoDup_disjoint in H0; eauto.
+Qed.
+
+Lemma free_allocas_preserves_wf_defs: forall maxb pinfo TD Mem lc' l0 als0 als Mem',
+  wf_defs maxb pinfo TD Mem lc' l0 als0 ->
+  NoDup (als ++ als0) ->
+  free_allocas TD Mem als = ret Mem' ->
+  wf_defs maxb pinfo TD Mem' lc' l0 als0.
+  (* This is only true if als is always disjoint with pinfo.id *) 
+Proof.
+  intros. unfold wf_defs in *. intros.
+  apply H in Hlkp; auto. clear H.
+  destruct Hlkp as [J1 J2]. 
+  split; eauto using free_allocas_preserves_wf_alloca.
+Qed.
+
+Lemma undef_disjoint_with_runtime_alloca: forall g td mb t1 t2
+  (Hc2g : ret g = gundef td t1),
+  no_alias g ($ blk2GV td mb # typ_pointer t2 $).
+Admitted.
+
+Lemma free_allocas_preserves_wf_lc: forall td Mem als Mem' lc,
+  wf_lc Mem lc -> free_allocas td Mem als = ret Mem' -> wf_lc Mem' lc.
+Admitted.
+
+Lemma returnUpdateLocals__wf_lc: forall maxb td Result (lc:DGVMap) gl c' 
+  lc' Mem lc''
+  (H1 : Opsem.returnUpdateLocals td c' Result lc lc' gl = ret lc'')
+  (Hwflc1 : wf_lc Mem lc) (Hwflc2 : wf_lc Mem lc')
+  (Hwfg : wf_globals maxb gl) (Hgbound : maxb < Mem.nextblock Mem),
+  wf_lc Mem lc''.
+Admitted.
+
+Lemma free_allocas_preserves_wf_ECStack: forall maxb pinfo td Mem als Mem' ECs,
+  wf_ECStack maxb pinfo td Mem ECs ->
+  free_allocas td Mem als = ret Mem' ->
+  NoDup (als ++ (flat_map
+                  (fun ec : Opsem.ExecutionContext =>
+                   let '{| Opsem.Allocas := als |} := ec in als)
+                   ECs)) ->
+  wf_ECStack maxb pinfo td Mem' ECs.
+Admitted.
+
+Lemma wf_ECStack_head_tail__inv: forall maxb pinfo TD M lc ec1 ecs2,
+  wf_ECStack_head_tail maxb pinfo TD M lc (ec1::ecs2) ->
+  wf_ECStack_head_tail maxb pinfo TD M lc ecs2.
+Admitted.
+
+Lemma free_allocas_preserves_wf_ECStack_head_tail : forall maxb pinfo td M M' 
+  lc als lc' F' lc'' ECs gl Result c',
+  free_allocas td M als = ret M' ->
+  Opsem.returnUpdateLocals td c' Result lc lc' gl = ret lc'' ->
+  wf_ECStack_head_tail maxb pinfo td M lc ((F', lc')::ECs) ->
+  wf_ECStack_head_tail maxb pinfo td M lc' ECs ->
+  wf_ECStack_head_tail maxb pinfo td M' lc'' ECs.
+Admitted.
+
+Lemma free_allocas_preserves_wf_Mem: forall maxb td Mem als Mem',
+  wf_Mem maxb td Mem -> free_allocas td Mem als = ret Mem' -> 
+  wf_Mem maxb td Mem'.
+Admitted.
+
+Lemma free_allocas_preserves_wf_als : forall maxb TD M M' als als0
+  (Hfree: free_allocas TD M als0 = ret M') 
+  (Hwf: wf_als maxb M als),
+  wf_als maxb M' als.
+Admitted.
+
+Lemma preservation_return_helper: forall (g : GVsT DGVs) pinfo lc' Mem'
+  als' td maxb Mem ECs lc gl t Result
+  (HeqR1 : ret g = Opsem.getOperandValue td Result lc gl)
+  (g0 : GVsT DGVs)
+  (HeqR2 : ret g0 = lift_op1 DGVs (fit_gv td t) g t)
+  (Hwfg : wf_globals maxb gl)
+  (l0 : list atom)
+  (Hfr1 : wf_ECStack_head_tail maxb pinfo td Mem lc
+           ((PI_f pinfo, lc')
+            :: List.map
+                 (fun ec : Opsem.ExecutionContext =>
+                  let '{| Opsem.CurFunction := f; Opsem.Locals := lc |} :=
+                       ec in (f, lc)) ECs))
+  (Hinscope2 : wf_defs maxb pinfo td Mem' lc' l0 als')
+  (gvsa : GVsT DGVs)
+  (Hpindom : In (PI_id pinfo) l0)
+  (Hlkp : lookupAL (GVsT DGVs) lc' (PI_id pinfo) = ret gvsa),
+  no_alias g0 gvsa.
+Proof.
+  intros.
+  assert (Hlkp':=Hlkp).
+  apply Hinscope2 in Hlkp'; auto.
+  destruct Hlkp' as [[[mb [EQ [Hin Hbound]]] _] _]; subst.
+  edestruct Hfr1 as [G _]; simpl; eauto.
+  clear Hfr1.
+  simpl in G.
+  Local Transparent lift_op1. simpl in HeqR2.
+  unfold MDGVs.lift_op1, fit_gv in HeqR2.
+  destruct (getTypeSizeInBits td t); tinv HeqR2.
+  destruct (sizeGenericValue g =n= nat_of_Z (ZRdiv (Z_of_nat n) 8)).
+    inv HeqR2.
+    destruct Result; simpl in HeqR1; eauto.            
+    eapply wf_globals_disjoint_with_runtime_alloca; eauto.
+  
+    eapply undef_disjoint_with_runtime_alloca; eauto.
+Qed.
+
+Lemma wf_als_split: forall maxb M als als',
+  wf_als maxb M (als++als') -> wf_als maxb M als /\ wf_als maxb M als'.
+Proof.
+  intros.
+  destruct H as [J1 J2].
+  apply NoDup_split in J1.
+  destruct J1 as [J11 J12].
+  split.
+    split; auto.
+      intros. apply J2. apply in_or_app; auto.
+    split; auto.
+      intros. apply J2. apply in_or_app; auto.
+Qed.
+
+Ltac SSSSSCase name := Case_aux subsubsubsubsubcase name.
+Ltac SSSSSSCase name := Case_aux subsubsubsubsubsubcase name.
+
+Lemma preservation_return : forall maxb pinfo (HwfPI : WF_PhiInfo pinfo)  
+  F B rid RetTy Result lc F' B' c' cs' tmn' lc' EC Mem als als' cfg
+  EC1 EC2 (Hwfg: wf_globals maxb (OpsemAux.Globals cfg))
+  (EQ1:EC1 = {| Opsem.CurFunction := F;
+                Opsem.CurBB := B;
+                Opsem.CurCmds := nil;
+                Opsem.Terminator := insn_return rid RetTy Result;
+                Opsem.Locals := lc;
+                Opsem.Allocas := als |})
+  (EQ2:EC2 = {| Opsem.CurFunction := F';
+                Opsem.CurBB := B';
+                Opsem.CurCmds := c' :: cs';
+                Opsem.Terminator := tmn';
+                Opsem.Locals := lc';
+                Opsem.Allocas := als' |})
+  (Hinv : OpsemPP.wf_State cfg
+           {| Opsem.ECS := EC1 :: EC2 :: EC;
+              Opsem.Mem := Mem |})
+  Mem' lc'' (H : Instruction.isCallInst c' = true)
+  (H0 : free_allocas (OpsemAux.CurTargetData cfg) Mem als = ret Mem')
+  (H1 : Opsem.returnUpdateLocals 
+          (OpsemAux.CurTargetData cfg) c' 
+            Result lc lc' (OpsemAux.Globals cfg) = ret lc'')
+  (HwfS1 : wf_State maxb pinfo cfg
+            {| Opsem.ECS := EC1 :: EC2 :: EC;
+               Opsem.Mem := Mem |}),
+  wf_State maxb pinfo cfg
+     {| Opsem.ECS :=
+             {| Opsem.CurFunction := F';
+                Opsem.CurBB := B';
+                Opsem.CurCmds := cs';
+                Opsem.Terminator := tmn';
+                Opsem.Locals := lc'';
+                Opsem.Allocas := als' |} :: EC;
+        Opsem.Mem := Mem' |}.
+Proof.
+Local Opaque inscope_of_tmn inscope_of_cmd.
+
+  intros. subst. destruct cfg as [S [los nts] Ps gl fs].
+  destruct Hinv as 
+    [_ [HwfSystem [HmInS [Hnonempty [
+     [Hreach1 [HBinF1 [HFinPs1 [_ [_ [l1 [ps1 [cs1' Heq1]]]]]]]] 
+     [
+       [
+         [Hreach2 [HBinF2 [HFinPs2 [_ [_ [l2 [ps2 [cs2' Heq2]]]]]]]]
+         [HwfEC0 HwfCall]
+       ]
+       HwfCall'
+     ]
+    ]]]]]; subst.
+  fold (@OpsemPP.wf_ECStack DGVs) in HwfEC0.
+  destruct HwfS1 as 
+    [
+      [[Hinscope1 Hwflc1] [[[Hinscope2 Hwflc2] [HwfECs Hfr2]] Hfr1]] 
+      [Hdisjals HwfM]
+    ]. simpl. simpl in Hdisjals.
+  fold wf_ECStack in HwfECs.
+  assert (Hdisjals':=Hdisjals).
+  destruct Hdisjals' as [Hdisjals' _].
+  split.
+  SCase "wf_ECStack".
+    split.
+    SSCase "wf_EC".
+    split.
+    SSSCase "sdom".
+
+    destruct (fdef_dec (PI_f pinfo) F'); subst; auto.
+    remember (inscope_of_cmd 
+      (PI_f pinfo) (block_intro l2 ps2 (cs2' ++ c' :: cs') tmn') c') as R2.
+    destruct R2; try solve [inversion Hinscope2].
+(*
+    remember (inscope_of_tmn F
+               (block_intro l1 ps1 (cs1' ++ nil)(insn_return rid RetTy Result))
+               (insn_return rid RetTy Result)) as R1. 
+    destruct R1; try solve [inversion Hinscope1].
+*)
+    remember (getCmdID c') as R.
+    destruct c'; try solve [inversion H].
+    assert (In (insn_call i0 n c t v p) 
+      (cs2'++[insn_call i0 n c t v p] ++ cs')) as HinCs.
+      apply in_or_app. right. simpl. auto.
+    assert (Hwfc := HBinF2).
+    eapply wf_system__wf_cmd with (c:=insn_call i0 n c t v p) in Hwfc; eauto.
+    assert (wf_fdef nil S (module_intro los nts Ps) (PI_f pinfo)) as HwfF.
+      eapply wf_system__wf_fdef; eauto.
+    assert (uniqFdef (PI_f pinfo)) as HuniqF.
+      eapply wf_system__uniqFdef; eauto.
+
+    assert (NoDup (als ++ als')) as Hnodup.
+      rewrite_env 
+        ((als ++ als') ++ 
+          flat_map
+            (fun ec : Opsem.ExecutionContext =>
+             let '{| Opsem.Allocas := als |} := ec in als) EC) in Hdisjals'.
+      apply NoDup_split in Hdisjals'.
+      destruct Hdisjals'; auto.
+    eapply free_allocas_preserves_wf_defs in Hinscope2; eauto. clear Hnodup.
+    destruct cs'.
+    SSSSCase "cs' = nil".
+      assert (~ In (getCmdLoc (insn_call i0 n c t v p)) (getCmdsLocs cs2')) 
+        as Hnotin.
+        eapply wf_system__uniq_block with (f:=(PI_f pinfo)) in HwfSystem; eauto.        
+        simpl in HwfSystem.
+        apply NoDup_inv in HwfSystem.
+        destruct HwfSystem as [_ J].
+        apply NoDup_inv in J.
+        destruct J as [J _].
+        rewrite getCmdsLocs_app in J.
+        simpl in J.
+        apply NoDup_last_inv in J. auto.
+      assert (HeqR2':=HeqR2).
+      apply inscope_of_cmd_tmn in HeqR2; auto.
+      destruct HeqR2 as [ids2 [J1 J2]].
+      simpl_env. rewrite <- J1.
+      unfold Opsem.returnUpdateLocals in H1. simpl in H1.
+      remember (Opsem.getOperandValue (los,nts) Result lc gl) as R1.
+      destruct R1; try solve [inv H1].
+      destruct R.
+      SSSSSCase "c' defines a variable".
+        destruct n; inv HeqR.
+        destruct t; tinv H1.
+
+        remember (MDGVs.lift_op1 (fit_gv (los, nts) t) g t) as R2.
+        destruct R2; inv H1.
+
+        apply wf_defs_updateAddAL with (ids1:=l0); auto.
+          split.
+            eapply preservation_return_helper; eauto.
+
+            intro; subst.
+            admit. (* PI_id pinfo cannot be of an id for callsite *) 
+
+      SSSSSCase "c' defines nothing".
+        destruct n; inv HeqR. inv H1.
+        simpl in J2.
+        eapply wf_defs_eq; eauto. 
+        
+    SSSSCase "cs' <> nil".
+      assert (NoDup (getCmdsLocs (cs2' ++ [insn_call i0 n c t v p] ++ [c0] ++ 
+        cs'))) as Hnodup.
+        eapply wf_system__uniq_block with (f:=PI_f pinfo) in HwfSystem; eauto.
+        simpl in HwfSystem.
+        apply NoDup_inv in HwfSystem.
+        destruct HwfSystem as [_ J].
+        apply NoDup_inv in J.
+        destruct J as [J _]. auto.
+      assert (HeqR2':=HeqR2). simpl_env in HeqR2.
+      apply inscope_of_cmd_cmd in HeqR2; auto.
+      destruct HeqR2 as [ids2 [J1 J2]].        
+      simpl_env. rewrite <- J1.
+      unfold Opsem.returnUpdateLocals in H1. simpl in H1.
+      remember (Opsem.getOperandValue (los,nts) Result lc gl) as R1.
+      destruct R1; try solve [inv H1].
+      destruct R.
+      SSSSSCase "c' defines a variable".
+        destruct n; inv HeqR.
+        destruct t; tinv H1.
+        remember (MDGVs.lift_op1 (fit_gv (los, nts) t) g t) as R2.
+        destruct R2; inv H1.
+        inv Hwfc. inv H16. inv H7. inv H18.
+
+        apply wf_defs_updateAddAL with (ids1:=l0); auto.
+          split.
+            eapply preservation_return_helper; eauto.
+
+            intro; subst.
+            admit. (* PI_id pinfo cannot be of an id for callsite *) 
+
+      SSSSSCase "c' defines nothing".
+        destruct n; inv HeqR. inv H1.
+        simpl in J2.
+        eapply wf_defs_eq; eauto. 
+
+      SSSCase "wflc".
+        clear - Hwflc1 Hwflc2 H1 Hwfg HwfM H0.
+        eapply free_allocas_preserves_wf_lc in H0; eauto.
+        destruct HwfM.
+        eapply returnUpdateLocals__wf_lc in H1; eauto.
+
+    split.
+    SSCase "wf_ECs".
+      eapply free_allocas_preserves_wf_ECStack; eauto.
+      apply NoDup_strenthening in Hdisjals'; auto.
+
+    SSCase "wf_ECs_head_tail".
+      simpl in Hfr1, Hfr2.
+      eapply free_allocas_preserves_wf_ECStack_head_tail; eauto.
+
+  split.
+  SCase "Disjoint Allocas".
+    apply wf_als_split in Hdisjals.
+    destruct Hdisjals; auto.
+    eapply free_allocas_preserves_wf_als; eauto.
+
+  SCase "wfM".
+    eapply free_allocas_preserves_wf_Mem; eauto.
+
+Transparent inscope_of_tmn inscope_of_cmd.
+Qed.
+
+Ltac unfold_blk2GV := unfold blk2GV, ptr2GV, val2GV.
+
+Lemma gptr_spec: forall pinfo gv3 mb td
+  (Hwfgv : ~
+          (exists blk : Values.block,
+             exists ofs : int32, gv3 = mk_gptr blk ofs)),
+  gv3 <> $ blk2GV td mb # typ_pointer (PI_typ pinfo) $.
+Proof.
+  intros. destruct td.
+  intro J. subst. apply Hwfgv.
+  unfold_blk2GV. unfold mk_gptr.
+Local Transparent gv2gvs.
+  unfold gv2gvs. simpl. unfold MDGVs.gv2gvs. eauto.
+Opaque gv2gvs. 
+Qed.
+
+Lemma updateAddAL__wf_lc: forall gv3 Mem0 lc id0
+  (Hwfgv: forall blk ofs, gv3 = mk_gptr blk ofs -> blk < Mem.nextblock Mem0)
+  (Hwflc: wf_lc Mem0 lc),
+  wf_lc Mem0 (updateAddAL (GVsT DGVs) lc id0 gv3).
+Proof.
+  intros. unfold wf_lc in *. intros.
+  destruct (id_dec id0 id1); subst.
+    rewrite lookupAL_updateAddAL_eq in H; auto. inv H. eauto.
+
+    rewrite <- lookupAL_updateAddAL_neq in H; auto.
+    eapply Hwflc; eauto.
+Qed.
+
+Lemma updateAddAL__wf_ECStack_head_tail: forall maxb pinfo td M lc ECs
+  id0 gv3 
+  (Hwfgv: forall blk ofs, gv3 = mk_gptr blk ofs -> blk < Mem.nextblock M),
+  wf_ECStack_head_tail maxb pinfo td M lc ECs ->
+  wf_ECStack_head_tail maxb pinfo td M (updateAddAL (GVsT DGVs) lc id0 gv3) ECs.
+Admitted.
+
+Definition wf_GVs_in_EC (maxb:Values.block) (pinfo:PhiInfo) TD M 
+  (ec:Opsem.ExecutionContext)(id1:id)(gv1:GVsT DGVs) : Prop :=
+let '(Opsem.mkEC f b cs tmn lc als) := ec in
+(if (fdef_dec (PI_f pinfo) f) then 
+  match cs with
+  | nil => 
+    match inscope_of_tmn f b tmn with
+    | Some ids => wf_GVs maxb pinfo TD M lc ids als id1 gv1
+    | None => False
+    end
+  | c::_ =>
+    match inscope_of_cmd f b c with
+    | Some ids => wf_GVs maxb pinfo TD M lc ids als id1 gv1
+    | None => False
+    end
+  end 
+else True) /\
+(forall blk ofs, gv1 = mk_gptr blk ofs -> blk < Mem.nextblock M).
+
+Lemma preservation_pure_cmd_updated_case : forall (F : fdef)(B : block)
+  (lc : DGVMap)(gv3 : GVsT DGVs) (cs : list cmd) (tmn : terminator) id0 c0 Mem0 
+  als ECs pinfo 
+  (HwfPI : WF_PhiInfo pinfo) (Hid : Some id0 = getCmdID c0) cfg maxb
+  EC
+  (Heq: EC = {| Opsem.CurFunction := F;
+                Opsem.CurBB := B;
+                Opsem.CurCmds := c0 :: cs;
+                Opsem.Terminator := tmn;
+                Opsem.Locals := lc;
+                Opsem.Allocas := als |})
+  (Hwfgv : wf_GVs_in_EC maxb pinfo (OpsemAux.CurTargetData cfg) Mem0 EC id0 gv3)
+  (Hinv : OpsemPP.wf_State cfg
+           {| Opsem.ECS := EC :: ECs;
+              Opsem.Mem := Mem0 |})
+  (HwfS1 : wf_State maxb pinfo cfg
+            {| Opsem.ECS := EC :: ECs;
+               Opsem.Mem := Mem0 |}),
+   wf_State maxb pinfo cfg
+     {|
+     Opsem.ECS := {|
+            Opsem.CurFunction := F;
+            Opsem.CurBB := B;
+            Opsem.CurCmds := cs;
+            Opsem.Terminator := tmn;
+            Opsem.Locals := updateAddAL (GVsT DGVs) lc id0 gv3;
+            Opsem.Allocas := als |} :: ECs;
+     Opsem.Mem := Mem0 |}.
+Proof.
+Local Opaque inscope_of_cmd inscope_of_tmn.
+
+  intros. subst. destruct Hwfgv as [Hwfgv1 Hwfgv2].
+  destruct cfg as [S [los nts] Ps gl fs].
+  destruct Hinv as 
+    [_ [HwfSystem [HmInS [Hnonempty [
+     [Hreach1 [HBinF1 [HFinPs1 [_ [_ [l1 [ps1 [cs1' Heq1]]]]]]]] 
+     [HwfEC0 HwfCall]
+    ]]]]]; subst.
+  fold (@OpsemPP.wf_ECStack DGVs) in HwfEC0.
+  destruct HwfS1 as 
+    [[[Hinscope1 Hwflc1] [HwfECs Hfr2]] [Hdisjals HwfM]].
+  simpl. simpl in Hdisjals.
+  fold wf_ECStack in HwfECs.
+  simpl in Hwfgv1.
+  split; auto.
+  SCase "wf_ECStack".
+    split.
+    SSCase "wf_EC".
+    split.
+    SSSCase "sdom".
+    destruct (fdef_dec (PI_f pinfo) F); subst; auto.
+
+  remember (inscope_of_cmd (PI_f pinfo) 
+    (block_intro l1 ps1 (cs1' ++ c0 :: cs) tmn) c0) as R1. 
+  assert (HeqR1':=HeqR1).
+
+Transparent inscope_of_cmd.
+
+  unfold inscope_of_cmd, inscope_of_id in HeqR1'.
+  assert (uniqFdef (PI_f pinfo)) as HuniqF.
+    eapply wf_system__uniqFdef; eauto.
+  destruct R1; try solve [inversion Hinscope1].
+  repeat (split; try solve [auto]).
+      assert (Hid':=Hid).
+      symmetry in Hid.
+      apply getCmdLoc_getCmdID in Hid.
+      subst.
+      assert (cmdInBlockB c0 (block_intro l1 ps1 (cs1' ++ c0 :: cs) tmn) = true) 
+        as Hin.
+        simpl. apply In_InCmdsB. apply in_middle.
+      destruct cs; simpl_env in *.
+      SSSSCase "cs = nil".
+        assert (~ In (getCmdLoc c0) (getCmdsLocs cs1')) as Hnotin.
+          (* this lemma should be lifted to the top *)
+          eapply wf_system__uniq_block with (f:=PI_f pinfo) in HwfSystem; eauto.
+          simpl in HwfSystem.
+          apply NoDup_inv in HwfSystem.
+          destruct HwfSystem as [_ J].
+          apply NoDup_inv in J.
+          destruct J as [J _].
+          rewrite getCmdsLocs_app in J.
+          simpl in J.
+          apply NoDup_last_inv in J. auto.
+
+        apply inscope_of_cmd_tmn in HeqR1; auto.
+        destruct HeqR1 as [ids2 [J1 J2]].        
+        rewrite <- J1.
+        assert (In c0 (cs1' ++ [c0])) as HinCs.
+          apply in_or_app. right. simpl. auto.
+        assert (Hwfc := HBinF1).
+        eapply wf_system__wf_cmd with (c:=c0) in Hwfc; 
+          eauto.
+        rewrite <- Hid' in J2.
+        assert (HwfF:=HFinPs1). eapply wf_system__wf_fdef in HwfF; eauto.
+        eapply wf_defs_updateAddAL; eauto.
+
+      SSSSCase "cs <> nil".
+        assert (NoDup (getCmdsLocs (cs1' ++ [c0] ++ [c] ++ cs))) as Hnodup.
+          (* this lemma should be lifted to the top *)
+          eapply wf_system__uniq_block with (f:=PI_f pinfo) in HwfSystem; eauto.
+          simpl in HwfSystem.
+          apply NoDup_inv in HwfSystem.
+          destruct HwfSystem as [_ J].
+          apply NoDup_inv in J.
+          destruct J as [J _]. auto.
+        apply inscope_of_cmd_cmd in HeqR1; auto.
+        destruct HeqR1 as [ids2 [J1 J2]].        
+        rewrite <- J1.
+        assert (In c0 (cs1' ++ [c0] ++ [c] ++ cs)) as HinCs.
+          apply in_or_app. right. simpl. auto.
+        assert (Hwfc := HBinF1).
+        eapply wf_system__wf_cmd with (c:=c0) in Hwfc; 
+          eauto.
+        rewrite <- Hid' in J2.
+        assert (HwfF:=HFinPs1). eapply wf_system__wf_fdef in HwfF; eauto.
+        eapply wf_defs_updateAddAL; eauto.
+
+      SSSCase "wflc".
+        apply updateAddAL__wf_lc; auto.
+
+    split; auto.
+    SSCase "wf_ECs_head_tail".
+      simpl in Hfr2.
+      eapply updateAddAL__wf_ECStack_head_tail; eauto.
+
+Transparent inscope_of_cmd inscope_of_tmn.
+
+Qed.
+
+Lemma BOP__wf_GVs_in_EC : forall (v : value) (v0 : value) (id1 : id) (bop0 : bop)
+  gvs3 TD bop0 sz0 lc gl EC Mem0 td pinfo maxb
+  (H11 : BOP TD lc gl bop0 sz0 v v0 = ret gvs3),
+  wf_GVs_in_EC maxb pinfo td Mem0 EC id1 gvs3.
+Proof.
+  intros. 
+Admitted.
+
+Lemma CAST__wf_GVs_in_EC : forall (v : value) (v0 : value) (id1 : id)
+  gvs2 TD lc gl EC Mem0 td pinfo maxb castop0 t1 v1 t2
+  (H11 : Opsem.CAST TD lc gl castop0 t1 v1 t2 = ret gvs2),
+  wf_GVs_in_EC maxb pinfo td Mem0 EC id1 gvs2.
+Proof.
+  intros. 
+Admitted.
+
+Lemma malloc_preserves_wf_ECStack_head_tail : forall maxb pinfo ECs TD M tsz gn 
+  align0 M' lc mb t id0,
+  malloc TD M tsz gn align0 = ret (M', mb) ->
+  wf_ECStack_head_tail maxb pinfo TD M lc ECs ->
+  wf_ECStack_head_tail maxb pinfo TD M' 
+    (updateAddAL (GVsT DGVs) lc id0
+        ($ blk2GV TD mb # typ_pointer t $)) ECs.
+Admitted.
+
+Lemma malloc_preserves_wf_ECStack : forall maxb pinfo ECs TD M tsz gn align0 M' 
+  mb,
+  malloc TD M tsz gn align0 = ret (M', mb) ->
+  wf_ECStack maxb pinfo TD M ECs ->
+  wf_ECStack maxb pinfo TD M' ECs.
+Admitted.
+
+Lemma malloc_preserves_wf_EC : forall maxb pinfo TD M tsz gn align0 M' mb 
+  als t id0 F B cs tmn lc v gns gl
+  (H : getTypeAllocSize TD t = ret tsz)
+  (H0 : Opsem.getOperandValue TD v lc gl = ret gns)
+  (H1 : gn @ gns)
+  (H2 : malloc TD M tsz gn align0 = ret (M', mb))
+  (HwfEC: wf_ExecutionContext maxb pinfo TD M 
+            {| Opsem.CurFunction := F;
+               Opsem.CurBB := B;
+               Opsem.CurCmds := insn_malloc id0 t v align0 :: cs;
+               Opsem.Terminator := tmn;
+               Opsem.Locals := lc;
+               Opsem.Allocas := als |}),
+  wf_ExecutionContext maxb pinfo TD M'
+   {| Opsem.CurFunction := F;
+      Opsem.CurBB := B;
+      Opsem.CurCmds := cs;
+      Opsem.Terminator := tmn;
+      Opsem.Locals := updateAddAL (GVsT DGVs) lc id0
+                        ($ blk2GV TD mb # typ_pointer t $);
+      Opsem.Allocas := als |}.
+Admitted.
+
+Lemma malloc_preserves_wf_Mem : forall maxb TD M tsz gn align0 M' mb,
+  malloc TD M tsz gn align0 = ret (M', mb) ->
+  wf_Mem maxb TD M ->
+  wf_Mem maxb TD M'.
+Admitted.
+
+Lemma wf_EC__wf_lc : forall maxb pinfo TD M EC,
+  wf_ExecutionContext maxb pinfo TD M EC ->
+  wf_lc M (Opsem.Locals EC).
+Admitted.
+
+Lemma alloca_preserves_wf_EC : forall maxb pinfo TD M tsz gn align0 M' mb 
+  als t id0 F B cs tmn lc v gns gl
+  (H : getTypeAllocSize TD t = ret tsz)
+  (H0 : Opsem.getOperandValue TD v lc gl = ret gns)
+  (H1 : gn @ gns)
+  (H2 : malloc TD M tsz gn align0 = ret (M', mb))
+  (HwfEC: wf_ExecutionContext maxb pinfo TD M 
+            {| Opsem.CurFunction := F;
+               Opsem.CurBB := B;
+               Opsem.CurCmds := insn_malloc id0 t v align0 :: cs;
+               Opsem.Terminator := tmn;
+               Opsem.Locals := lc;
+               Opsem.Allocas := als |}),
+  wf_ExecutionContext maxb pinfo TD M'
+   {| Opsem.CurFunction := F;
+      Opsem.CurBB := B;
+      Opsem.CurCmds := cs;
+      Opsem.Terminator := tmn;
+      Opsem.Locals := updateAddAL (GVsT DGVs) lc id0
+                        ($ blk2GV TD mb # typ_pointer t $);
+      Opsem.Allocas := mb :: als |}.
+Admitted.
+
+Lemma malloc_preserves_wf_als : forall maxb TD M M' tsz gn align0 mb als
+  (Hmalloc: malloc TD M tsz gn align0 = ret (M', mb)) 
+  (Hwf: wf_als maxb M als),
+  wf_als maxb M' (mb::als).
+Admitted.
+
+Lemma mload__wf_GVs_in_EC : forall (v : value) (v0 : value) (id1 : id) 
+  gvs3 TD t align0 (lc:DGVMap) gl EC Mem td pinfo maxb mp mps
+  (Hwflc: wf_lc Mem lc) (Hwfgl: wf_globals maxb gl)
+  (H : Opsem.getOperandValue td v lc gl = ret mps)
+  (H0 : mp @ mps)
+  (H1 : mload TD Mem mp t align0 = ret gvs3),
+  wf_GVs_in_EC maxb pinfo td Mem EC id1 gvs3.
+Proof.
+  intros. 
+Admitted.
+
+Lemma mstore_preserves_wf_ECStack_head_tail : forall maxb pinfo ECs TD M 
+  gv1 align M' lc mp2 t,
+  mstore TD M mp2 t gv1 align = Some M' ->
+  wf_ECStack_head_tail maxb pinfo TD M lc ECs ->
+  wf_ECStack_head_tail maxb pinfo TD M' lc ECs.
+Admitted.
+
+Lemma mstore_preserves_wf_ECStack : forall maxb pinfo ECs TD M mp2 t gv1 align 
+  M', 
+  mstore TD M mp2 t gv1 align = Some M' ->
+  wf_ECStack maxb pinfo TD M ECs ->
+  wf_ECStack maxb pinfo TD M' ECs.
+Admitted.
+
+Lemma mstore_preserves_wf_EC : forall maxb pinfo TD M v1 gvs1 gv1 M'
+  als t id0 F B cs tmn (lc:DGVMap) gl align0 v2 mp2
+  (Hwflc: wf_lc M lc) (Hwfgl: wf_globals maxb gl)
+  (H0 : Opsem.getOperandValue TD v1 lc gl = Some gvs1)
+  (H1 : gv1 @ gvs1)
+  (H2 : mstore TD M mp2 t gv1 align0 = Some M')
+  (HwfEC: wf_ExecutionContext maxb pinfo TD M 
+            {| Opsem.CurFunction := F;
+               Opsem.CurBB := B;
+               Opsem.CurCmds := insn_store id0 t v1 v2 align0 :: cs;
+               Opsem.Terminator := tmn;
+               Opsem.Locals := lc;
+               Opsem.Allocas := als |}),
+  wf_ExecutionContext maxb pinfo TD M'
+   {| Opsem.CurFunction := F;
+      Opsem.CurBB := B;
+      Opsem.CurCmds := cs;
+      Opsem.Terminator := tmn;
+      Opsem.Locals := lc;
+      Opsem.Allocas := als |}.
+Admitted.
+
+Lemma mstore_preserves_wf_Mem : forall maxb TD M mp2 t gv1 align M',
+  mstore TD M mp2 t gv1 align = Some M' ->
+  wf_Mem maxb TD M ->
+  wf_Mem maxb TD M'.
+Admitted.
+
+Lemma mstore_preserves_wf_als : forall TD M mp2 t gv1 align M' maxb als
+  (Hst: mstore TD M mp2 t gv1 align = Some M') 
+  (Hwf: wf_als maxb M als),
+  wf_als maxb M' als.
+Admitted.
+
+Lemma GEP__wf_GVs_in_EC : forall (v : value) (v0 : value) (id1 : id) 
+  mp' TD t (lc:DGVMap) gl EC Mem td pinfo maxb (mp:GVsT DGVs) mps 
+  inbounds0 vidxs (Hwflc: wf_lc Mem lc) (Hwfgl: wf_globals maxb gl)
+  (H : Opsem.getOperandValue td v lc gl = ret mps)
+  (H0 : mp @ mps)
+  (H1 : Opsem.GEP TD t mp vidxs inbounds0 = ret mp'),
+  wf_GVs_in_EC maxb pinfo td Mem EC id1 mp'.
+Proof.
+  intros. 
+Admitted.
+
+Lemma initLocals_preserves_wf_ECStack_head_tail: forall Mem (lc:DGVMap) maxb TD 
+  F ECs lc' gl (Hwflc1 : wf_lc Mem lc) pinfo gvs la lp
+  (Hwfg : wf_globals maxb gl)
+  (H3 : Opsem.params2GVs TD lp lc gl = ret gvs)
+  (H4 : Opsem.initLocals TD la gvs = ret lc')
+  (Hfr2 : wf_ECStack_head_tail maxb pinfo TD Mem lc
+            (List.map
+               (fun ec : Opsem.ExecutionContext =>
+                let '{| Opsem.CurFunction := f; Opsem.Locals := lc |} := ec in
+                  (f, lc)) ECs)),
+  wf_ECStack_head_tail maxb pinfo TD Mem lc'
+    ((F, lc)
+      :: List.map
+           (fun ec : Opsem.ExecutionContext =>
+            let '{| Opsem.CurFunction := f; Opsem.Locals := lc0 |} := ec in
+              (f, lc0)) ECs).
+Admitted.
+
+Lemma preservation_dbCall_case : forall fid fa rt la va lb gvs los
+  nts ifs s lc Ps Mem TD pinfo maxb
+  (Huniq: uniqFdef (fdef_intro (fheader_intro fa rt fid la va) lb))
+  (HwfF: wf_fdef ifs s (module_intro los nts Ps) 
+    (fdef_intro (fheader_intro fa rt fid la va) lb))
+  (HwfM : wf_Mem maxb TD Mem)
+  (Hinit : Opsem.initLocals TD la gvs = Some lc),
+  wf_defs maxb pinfo TD Mem lc (getArgsIDs la) nil.
+Proof.
+Admitted.
+
+Lemma initLocals_preserves_wf_lc: forall Mem (lc:DGVMap) maxb TD 
+  lc' gl (Hwflc1 : wf_lc Mem lc) gvs la lp
+  (Hwfg : wf_globals maxb gl)
+  (H3 : Opsem.params2GVs TD lp lc gl = ret gvs)
+  (H4 : Opsem.initLocals TD la gvs = ret lc')
+  (Hfr2 : wf_lc Mem lc),
+  wf_lc Mem lc'.
+Admitted.
+
+Lemma callExternalProc_preserves_wf_ECStack_head_tail : forall maxb pinfo   
+  ECs TD M M' (lc:DGVMap) gvs gvss fid oresult gl lp
+  (Hwflc: wf_lc M lc) (Hwfgl: wf_globals maxb gl) (H3 : gvs @@ gvss),
+  Opsem.params2GVs TD lp lc gl = ret gvss ->
+  OpsemAux.callExternalFunction M fid gvs = ret (oresult, M') ->
+  wf_ECStack_head_tail maxb pinfo TD M lc ECs ->
+  wf_ECStack_head_tail maxb pinfo TD M' lc ECs.
+Admitted.
+
+Lemma callExternalFunction_preserves_wf_ECStack : forall maxb pinfo ECs TD M  
+  M' gvs fid oresult, 
+  OpsemAux.callExternalFunction M fid gvs = ret (oresult, M') ->
+  wf_ECStack maxb pinfo TD M ECs ->
+  wf_ECStack maxb pinfo TD M' ECs.
+Admitted.
+
+Lemma callExternalProc_preserves_wf_EC : forall maxb pinfo TD M M' rid
+  als F B cs tmn gl gvss gvs fid oresult lp (lc:DGVMap) fv ft ca
+  (Hwflc: wf_lc M lc) (Hwfgl: wf_globals maxb gl) (H3 : gvs @@ gvss)
+  (J1: Opsem.params2GVs TD lp lc gl = ret gvss)
+  (J2: OpsemAux.callExternalFunction M fid gvs = ret (oresult, M'))
+  (HwfEC: wf_ExecutionContext maxb pinfo TD M 
+            {| Opsem.CurFunction := F;
+               Opsem.CurBB := B;
+               Opsem.CurCmds := insn_call rid true ca ft fv lp :: cs;
+               Opsem.Terminator := tmn;
+               Opsem.Locals := lc;
+               Opsem.Allocas := als |}),
+  wf_ExecutionContext maxb pinfo TD M'
+   {| Opsem.CurFunction := F;
+      Opsem.CurBB := B;
+      Opsem.CurCmds := cs;
+      Opsem.Terminator := tmn;
+      Opsem.Locals := lc;
+      Opsem.Allocas := als |}.
+Admitted.
+
+Lemma callExternalFunction_preserves_wf_Mem : forall maxb TD M fid gvs M' 
+  oresult,
+  OpsemAux.callExternalFunction M fid gvs = ret (oresult, M') ->
+  wf_Mem maxb TD M ->
+  wf_Mem maxb TD M'.
+Admitted.
+
+Lemma callExternalFunction_preserves_wf_als : forall M gvs M' maxb als fid 
+  oresult
+  (Hexcall: OpsemAux.callExternalFunction M fid gvs = ret (oresult, M')) 
+  (Hwf: wf_als maxb M als),
+  wf_als maxb M' als.
+Admitted.
+
+Lemma callExternalFun_preserves_wf_ECStack_head_tail : forall maxb pinfo   
+  ECs TD M M' (lc:DGVMap) gvs gvss fid result gl lp g0 rid ft
+  (Hwflc: wf_lc M lc) (Hwfgl: wf_globals maxb gl) (H3 : gvs @@ gvss)
+  (HeqR : ret g0 = fit_gv TD ft result),
+  Opsem.params2GVs TD lp lc gl = ret gvss ->
+  OpsemAux.callExternalFunction M fid gvs = ret (Some result, M') ->
+  wf_ECStack_head_tail maxb pinfo TD M lc ECs ->
+  wf_ECStack_head_tail maxb pinfo TD M' 
+    (updateAddAL (GVsT DGVs) lc rid ($ g0 # ft $)) ECs.
+Admitted.
+
+Lemma callExternalFun_preserves_wf_EC : forall maxb pinfo TD M M' rid
+  als F B cs tmn gl gvss gvs fid result lp (lc:DGVMap) fv ft ca g0
+  (Hwflc: wf_lc M lc) (Hwfgl: wf_globals maxb gl) (H3 : gvs @@ gvss)
+  (J1: Opsem.params2GVs TD lp lc gl = ret gvss)
+  (J2: OpsemAux.callExternalFunction M fid gvs = ret (Some result, M'))
+  (HeqR : ret g0 = fit_gv TD ft result)
+  (HwfEC: wf_ExecutionContext maxb pinfo TD M 
+            {| Opsem.CurFunction := F;
+               Opsem.CurBB := B;
+               Opsem.CurCmds := insn_call rid false ca ft fv lp :: cs;
+               Opsem.Terminator := tmn;
+               Opsem.Locals := lc;
+               Opsem.Allocas := als |}),
+  wf_ExecutionContext maxb pinfo TD M'
+   {| Opsem.CurFunction := F;
+      Opsem.CurBB := B;
+      Opsem.CurCmds := cs;
+      Opsem.Terminator := tmn;
+      Opsem.Locals := (updateAddAL (GVsT DGVs) lc rid ($ g0 # ft $));
+      Opsem.Allocas := als |}.
+Admitted.
+
+Lemma preservation : forall maxb pinfo cfg S1 S2 tr
+  (Hinv: OpsemPP.wf_State cfg S1)
+  (Hwfg: wf_globals maxb ((OpsemAux.Globals cfg)))
+  (HwfPI: WF_PhiInfo pinfo) (HsInsn: Opsem.sInsn cfg S1 S2 tr)
+  (HwfS1: wf_State maxb pinfo cfg S1), wf_State maxb pinfo cfg S2.
+Proof.
+  intros.
+  (sInsn_cases (induction HsInsn) Case); destruct TD as [los nts]; simpl HwfS1.
+
+Case "sReturn". eapply preservation_return; eauto. 
+Case "sReturnVoid". admit.
+Case "sBranch". admit.
+Case "sBranch_uncond". admit.
+Case "sBop".
+  eapply preservation_pure_cmd_updated_case in HwfS1; try solve [simpl; eauto]; 
+    eauto.
+    eapply BOP__wf_GVs_in_EC; eauto.
+Case "sFBop". admit.
+Case "sExtractValue". admit. 
+(* tricky case, 
+   we need to ensure that all extractable values cannot be aliased *)
+Case "sInsertValue". admit. 
+(* tricky case, 
+   we need to ensure that we are not inserting aliased values *)
+Case "sMalloc". 
+  destruct HwfS1 as [[HwfEC [HwfECs Hwfht]] [Hnonup1 HwfM1]].
+  split.
+    split.
+      eapply malloc_preserves_wf_EC in H2; eauto.
+    split.
+      eapply malloc_preserves_wf_ECStack in H2; eauto.
+      eapply malloc_preserves_wf_ECStack_head_tail in H2; eauto.
+  split.
+    eapply malloc_preserves_wf_als in H2; eauto.
+      simpl_env in H2.
+      apply wf_als_split in H2. destruct H2; auto.
+    eapply malloc_preserves_wf_Mem in H2; eauto.
+
+Case "sFree". 
+  destruct HwfS1 as [[HwfEC [HwfECs Hwfht]] [Hnonup1 HwfM1]].
+  assert (wf_lc Mem lc) as Hwflc.
+    apply wf_EC__wf_lc in HwfEC; auto.
+  split.
+    split.
+      eapply free_preserves_wf_EC in H1; eauto.
+    split.
+      eapply free_preserves_wf_ECStack in H1; eauto.
+      eapply free_preserves_wf_ECStack_head_tail in H1; eauto.
+  split.
+    eapply free_preserves_wf_als in H1; eauto.
+    eapply free_preserves_wf_Mem in H1; eauto.
+
+Case "sAlloca". 
+  destruct HwfS1 as [[HwfEC [HwfECs Hwfht]] [Hnonup1 HwfM1]].
+  split.
+    split.
+      eapply alloca_preserves_wf_EC in H2; eauto.
+    split.
+      eapply malloc_preserves_wf_ECStack in H2; eauto.
+      eapply malloc_preserves_wf_ECStack_head_tail in H2; eauto.
+  split.
+    eapply malloc_preserves_wf_als in H2; eauto.
+    eapply malloc_preserves_wf_Mem in H2; eauto.
+
+Case "sLoad". 
+  eapply preservation_pure_cmd_updated_case in HwfS1; try solve [simpl; eauto]; 
+    eauto.
+    destruct HwfS1 as [[[_ Hwflc] _] _]. 
+    eapply mload__wf_GVs_in_EC; eauto using wf_EC__wf_lc.
+
+Case "sStore". 
+  destruct HwfS1 as [[HwfEC [HwfECs Hwfht]] [Hnonup1 HwfM1]].
+  assert (wf_lc Mem lc) as Hwflc.
+    apply wf_EC__wf_lc in HwfEC; auto.
+  split.
+    split.
+      eapply mstore_preserves_wf_EC with (gvs1:=gvs1) in H3; eauto.
+    split.
+      eapply mstore_preserves_wf_ECStack in H3; eauto.
+      eapply mstore_preserves_wf_ECStack_head_tail in H3; eauto.
+  split.
+    eapply mstore_preserves_wf_als in H3; eauto.
+    eapply mstore_preserves_wf_Mem in H3; eauto.
+
+Case "sGEP". 
+  eapply preservation_pure_cmd_updated_case in HwfS1; try solve [simpl; eauto]; 
+    eauto.
+    destruct HwfS1 as [[[_ Hwflc] _] _]. 
+    eapply GEP__wf_GVs_in_EC; eauto using wf_EC__wf_lc.
+
+Case "sTrunc". admit.
+Case "sExt". admit.
+Case "sCast". 
+  eapply preservation_pure_cmd_updated_case in HwfS1; try solve [simpl; eauto]; 
+    eauto.
+    eapply CAST__wf_GVs_in_EC; eauto.
+
+Case "sIcmp". admit.
+Case "sFcmp". admit.
+Case "sSelect". admit. (* can return ptr *)
+Case "sCall". 
+Focus.
+  destruct Hinv as 
+    [_ [HwfSystem [HmInS [Hnonempty [
+     [Hreach1 [HBinF1 [HFinPs1 [_ [_ [l1 [ps1 [cs1' Heq1]]]]]]]] 
+     [HwfEC0 HwfCall]
+    ]]]]]; subst.
+  fold (@OpsemPP.wf_ECStack DGVs) in HwfEC0.
+  destruct HwfS1 as 
+    [[[Hinscope1 Hwflc1] [HwfECs Hfr2]] [Hdisjals HwfM]].
+  simpl in Hdisjals.
+  fold wf_ECStack in HwfECs.
+  assert (InProductsB (product_fdef (fdef_intro 
+    (fheader_intro fa rt fid la va) lb)) Ps = true) as HFinPs'.
+    apply OpsemAux.lookupFdefViaPtr_inversion in H1.
+    destruct H1 as [fn [H11 H12]].
+    eapply lookupFdefViaIDFromProducts_inv; eauto.
+  split; auto.
+  split.
+  SCase "1".     
+    assert (uniqFdef (fdef_intro (fheader_intro fa rt fid la va) lb)) as Huniq.
+      eapply wf_system__uniqFdef; eauto.
+    assert (wf_fdef nil S (module_intro los nts Ps) 
+      (fdef_intro (fheader_intro fa rt fid la va) lb)) as HwfF.
+      eapply wf_system__wf_fdef; eauto.
+    split.
+      destruct (fdef_dec (PI_f pinfo) 
+                 (fdef_intro (fheader_intro fa rt fid la va) lb)); auto.
+      assert (ps'=nil) as EQ.
+        eapply entryBlock_has_no_phinodes with (ifs:=nil)(s:=S); eauto.        
+      subst.
+      apply dom_entrypoint in H2. 
+      destruct cs'.
+        unfold inscope_of_tmn.
+        remember ((dom_analyze (fdef_intro (fheader_intro fa rt fid la va) lb)) 
+          !! l') as R.
+        destruct R. simpl in H2. subst. simpl.
+
+        eapply preservation_dbCall_case; eauto.
+
+        unfold inscope_of_cmd, inscope_of_id.
+        remember ((dom_analyze (fdef_intro (fheader_intro fa rt fid la va) lb)) 
+          !! l') as R.
+        destruct R. simpl. simpl in H2. subst. simpl.
+        destruct (eq_atom_dec (getCmdLoc c) (getCmdLoc c)) as [|n]; 
+          try solve [contradict n; auto]. 
+        eapply preservation_dbCall_case; eauto.
+
+      eapply initLocals_preserves_wf_lc; eauto.
+
+  split.
+    repeat (split; auto). 
+    simpl.
+    eapply initLocals_preserves_wf_ECStack_head_tail; eauto.
+Unfocus.
+
+Case "sExCall". 
+  destruct HwfS1 as [[HwfEC [HwfECs Hwfht]] [Hnonup1 HwfM1]].
+  assert (wf_lc Mem lc) as Hwflc.
+    apply wf_EC__wf_lc in HwfEC; auto.
+  unfold Opsem.exCallUpdateLocals in H5.
+  destruct noret0.
+    inv H5. 
+    split.
+      split.
+        eapply callExternalProc_preserves_wf_EC; eauto.
+      split.
+        eapply callExternalFunction_preserves_wf_ECStack; eauto.
+        eapply callExternalProc_preserves_wf_ECStack_head_tail; eauto.
+    split.
+      eapply callExternalFunction_preserves_wf_als; eauto.
+      eapply callExternalFunction_preserves_wf_Mem; eauto.
+
+    destruct oresult; inv H5.
+    destruct ft; tinv H7.
+    remember (fit_gv (los, nts) ft g) as R.
+    destruct R; inv H7.
+    split.
+      split.
+        eapply callExternalFun_preserves_wf_EC with (ca:=ca)(fv:=fv); eauto. 
+      split.
+        eapply callExternalFunction_preserves_wf_ECStack; eauto.
+        eapply callExternalFun_preserves_wf_ECStack_head_tail; eauto. 
+    split.
+      eapply callExternalFunction_preserves_wf_als; eauto.
+      eapply callExternalFunction_preserves_wf_Mem; eauto.
+Qed.
 
 (*****************************)
 (*
